compiler/dsl/coq/ReflexFin.v
@@ -1,22 +1,10 @@
+Require Import Arith.
+
 (* isomorphic to nats less than n *)
 Fixpoint fin (n : nat) : Type :=
   match n with
   | O => False
   | S n' => option (fin n')
-  end.
-
-Fixpoint opt_fin (bound : nat) (n : nat) : option (fin bound) :=
-  match bound with
-  | O => None
-  | S bound' =>
-    match n with
-    | O => Some None
-    | S n' =>
-      match opt_fin bound' n' with
-      | None => None
-      | Some fb' => Some (Some fb')
-      end
-    end
   end.
 
 Fixpoint nat_of_fin (bound : nat) (n : fin bound) :=
@@ -30,3 +18,20 @@ Fixpoint nat_of_fin (bound : nat) (n : fin bound) :=
   end n.
 
 Implicit Arguments nat_of_fin [bound].
+
+Fixpoint opt_fin (bound : nat) (n : nat)
+  : {f : fin bound & nat_of_fin f = n } + { n >= bound } :=
+  let ret b n := { f : fin b & nat_of_fin f = n } + { n >= b } in
+  match bound as _bound return ret _bound n with
+  | O => inright _ (le_0_n _)
+  | S bound' =>
+    match n as _n return ret (S bound') _n with
+    | O => inleft _ (existT _ None (eq_refl O))
+    | S n' =>
+      match opt_fin bound' n' with
+      | inleft (existT f' eq') =>
+        inleft _ (existT _ (Some f') (eq_ind_r (fun n => S n = S n') (eq_refl (S n')) eq'))
+      | inright pf => inright _ (le_n_S _ _ pf)
+      end
+    end
+  end.
